Finished STLC strong normalization proof with sum types added!!

theories/stlc.v
@@ -4,20 +4,21 @@ Require Import Relation_Operators.
 Require Import Autosubst.Autosubst.
 Require Import Lia.
 
-(* Some of the stuff about autosubst was taken from https://gist.github.com/tmoux/5027a9b9f6b5aee291d569e5f144b350 *)
+(* Some of the stuff about de Bruijn and the `autosubst` library was taken from https://gist.github.com/tmoux/5027a9b9f6b5aee291d569e5f144b350 *)
 
 Module STLC.
 
-  Open Scope nat_scope.
   Open Scope list_scope.
 
   Inductive tipe :=
   | Unit : tipe
   | Arrow : tipe -> tipe -> tipe
-  | Prod : tipe -> tipe -> tipe.
+  | Prod : tipe -> tipe -> tipe
+  | Sum : tipe -> tipe -> tipe.
 
   Notation " T '→' S " := (Arrow T S) (at level 99, right associativity).
-  Notation " T '×' S " := (Prod T S) (at level 98, left associativity).
+  Notation " T '×' S " := (Prod T S) (at level 97, left associativity).
+  Notation " T '⊕' S " := (Sum T S) (at level 98, left associativity).
 
   Inductive expr :=
   | Pair (e1 : expr) (e2 : expr)
@@ -25,6 +26,9 @@ Module STLC.
   | Abs (e : {bind expr})
   | Pi1 (e : expr)
   | Pi2 (e : expr)
+  | Inl (e : expr)
+  | Inr (e : expr)
+  | Case (e : expr) (e1 : {bind expr}) (e2 : {bind expr})
   | Var (x : var)
   | Null.
 
@@ -41,41 +45,48 @@ Module STLC.
   (* Empty context *)
   Notation "∅" := nil (at level 97).
 
-  (* Lemma lookup_cons_equal : forall Γ t t' n, lookup Γ n = Some t -> lookup (t' :: Γ) n = Some t. *)
-  (* Proof. *)
-  (*   intros. *)
-
+  Reserved Notation " Γ '⊢' e ':::' t " (at level 99).
   Inductive typing : context -> expr -> tipe -> Prop :=
   | prod_intro Γ e1 e2 t1 t2 : typing Γ e1 t1 -> typing Γ e2 t2 -> typing Γ (Pair e1 e2) (t1 × t2)
-  | prod_elim1 Γ e t1 t2 : typing Γ e (t1 × t2)  -> typing Γ (Pi1 e) t1
-  | prod_elim2 Γ e t1 t2 : typing Γ e (t1 × t2)  -> typing Γ (Pi2 e) t2
-  | arrow_intro Γ e t1 t2 : typing (t1 :: Γ) e t2 -> typing Γ (Abs e) (t1 → t2)
-  | arrow_elim Γ e1 e2 t1 t2 : typing Γ e1 (t1 → t2) -> typing Γ e2 t1 -> typing Γ (App e1 e2) t2
-  | unit_intro Γ : typing Γ Null Unit
-  | axiom_rule Γ n t : lookup Γ n = Some t -> typing Γ (Var n) t.
+  | prod_elim1 Γ e t1 t2 : Γ ⊢ e ::: (t1 × t2) -> Γ ⊢ (Pi1 e) ::: t1
+  | prod_elim2 Γ e t1 t2 : Γ ⊢ e ::: (t1 × t2) -> Γ ⊢ (Pi2 e) ::: t2
+  | arrow_intro Γ e t1 t2 : (t1 :: Γ) ⊢ e ::: t2 -> Γ ⊢ (Abs e) ::: (t1 → t2)
+  | arrow_elim Γ e1 e2 t1 t2 : Γ ⊢ e1 ::: (t1 → t2) -> Γ ⊢ e2 ::: t1 -> Γ ⊢ (App e1 e2) ::: t2
+  | sum_intro1 Γ e t1 t2 : Γ ⊢ e ::: t1 -> Γ ⊢ Inl e ::: t1 ⊕ t2
+  | sum_intro2 Γ e t1 t2 : Γ ⊢ e ::: t2 -> Γ ⊢ Inr e ::: t1 ⊕ t2
+  | sum_elim Γ e e1 e2 t1 t2 t3 : Γ ⊢ e ::: t1 ⊕ t2 -> t1 :: Γ ⊢ e1 ::: t3 -> t2 :: Γ ⊢ e2 ::: t3 -> Γ ⊢ Case e e1 e2 ::: t3
+  | unit_intro Γ : Γ ⊢ Null ::: Unit
+  | axiom_rule Γ n t : lookup Γ n = Some t -> Γ ⊢ (Var n) ::: t
+  where " Γ '⊢' e ':::' t " := (typing Γ e t).
   #[export] Hint Constructors typing : core.
-  Notation " Γ '⊢' e ':::' t " := (typing Γ e t) (at level 99).
 
   Inductive value : expr -> Prop :=
   | value_pair v1 v2 : value v1 -> value v2 -> value (Pair v1 v2)
+  | value_inl v : value v -> value (Inl v)
+  | value_inr v : value v -> value (Inr v)
   | value_abs e : value (Abs e)
   | value_null : value Null.
   #[export] Hint Constructors value : core.
 
   (** Small step CBV beta reduction *)
+  Reserved Notation " e '⇒' f " (at level 50).
   Inductive cbv_once : expr -> expr -> Prop :=
-  | cbv_pair1 e1 e2 e1' : cbv_once e1 e1' -> cbv_once (Pair e1 e2) (Pair e1' e2)
-  | cbv_pair2 e1 e2 e2' : cbv_once e2 e2' -> cbv_once (Pair e1 e2) (Pair e1 e2')
-  | cbv_pi1 e e' : cbv_once e e' -> cbv_once (Pi1 e) (Pi1 e')
-  | cbv_pi2 e e' : cbv_once e e' -> cbv_once (Pi2 e) (Pi2 e')
-  | cbv_val_pi1 v1 v2 : cbv_once (Pi1 (Pair v1 v2)) v1
-  | cbv_val_pi2 v1 v2 : cbv_once (Pi2 (Pair v1 v2)) v2
-  | cbv_fun e1 e2 e1' : cbv_once e1 e1' -> cbv_once (App e1 e2) (App e1' e2)
-  | cbv_arg e e2 e2' : cbv_once e2 e2' -> cbv_once (App (Abs e) e2) (App (Abs e) e2')
-  | cbv_sub e v : value v -> cbv_once (App (Abs e) v) (e.[v .: ids]).
+  | cbv_pair1 e1 e2 e1' : e1 ⇒ e1' -> (Pair e1 e2) ⇒ (Pair e1' e2)
+  | cbv_pair2 e1 e2 e2' : e2 ⇒ e2' -> (Pair e1 e2) ⇒ (Pair e1 e2')
+  | cbv_pi1 e e' : e ⇒ e' -> (Pi1 e) ⇒ (Pi1 e')
+  | cbv_pi2 e e' : e ⇒ e' -> (Pi2 e) ⇒ (Pi2 e')
+  | cbv_val_pi1 v1 v2 : (Pi1 (Pair v1 v2)) ⇒ v1
+  | cbv_val_pi2 v1 v2 : (Pi2 (Pair v1 v2)) ⇒ v2
+  | cbv_inl e e' : e ⇒ e' -> (Inl e) ⇒ (Inl e')
+  | cbv_inr e e' : e ⇒ e' -> (Inr e) ⇒ (Inr e')
+  | cbv_case e e' e1 e2 : e ⇒ e' -> Case e e1 e2 ⇒ Case e' e1 e2
+  | cbv_val_case_l v e1 e2 : Case (Inl v) e1 e2 ⇒ e1.[v .: ids]
+  | cbv_val_case_r v e1 e2 : Case (Inr v) e1 e2 ⇒ e2.[v .: ids]
+  | cbv_fun e1 e2 e1' : e1 ⇒ e1' -> (App e1 e2) ⇒ (App e1' e2)
+  | cbv_arg e e2 e2' : e2 ⇒ e2' -> (App (Abs e) e2) ⇒ (App (Abs e) e2')
+  | cbv_sub e v : value v -> (App (Abs e) v) ⇒ (e.[v .: ids])
+  where " e '⇒' f " := (cbv_once e f).
   #[export] Hint Constructors cbv_once : core.
-
-  Notation " e '⇒' f " := (cbv_once e f) (at level 21).
 
   (** Multi-step relation *)
   Definition cbv_multi := clos_refl_trans_n1 _ cbv_once.
@@ -119,6 +130,27 @@ Module STLC.
     - apply rtn1_trans with (y := Pi2 y); auto.
   Qed.
 
+  Lemma inl_steps_steps : forall e e', e ⇒* e' -> Inl e ⇒* Inl e'.
+  Proof.
+    intros e e' H. induction H.
+    - apply rtn1_refl.
+    - apply rtn1_trans with (y := Inl y); auto.
+  Qed.
+
+  Lemma inr_steps_steps : forall e e', e ⇒* e' -> Inr e ⇒* Inr e'.
+  Proof.
+    intros e e' H. induction H.
+    - apply rtn1_refl.
+    - apply rtn1_trans with (y := Inr y); auto.
+  Qed.
+
+  Lemma case_steps_steps : forall e e' e1 e2, e ⇒* e' -> Case e e1 e2 ⇒* Case e' e1 e2.
+  Proof.
+    intros e e' e1 e2 H. induction H.
+    - apply rtn1_refl.
+    - eapply rtn1_trans with (y := Case y e1 e2); auto.
+  Qed.
+
   Lemma app_fun_steps_steps : forall e e' e'', e ⇒* e' -> (App e e'') ⇒* (App e' e'').
   Proof.
     intros. induction H.
@@ -133,12 +165,16 @@ Module STLC.
     - apply rtn1_trans with (y := (App (Abs e) y)); auto.
   Qed.
 
+  (* Note: I wish we are using evaluation contexts... *)
+
+  (* The sum type logical relation is taken from page 15 of https://www.cs.uoregon.edu/research/summerschool/summer16/notes/AhmedLR.pdf*)
   Fixpoint V t v {struct t} : Prop :=
     let E t e : Prop := exists v, (cbv_multi e v) /\ (V t v) in
     match t with
     | Unit => v = Null
+    | Sum t1 t2 => (exists v1 : expr, v = Inl v1 /\ V t1 v1) \/ (exists v2 : expr, v = Inr v2 /\ V t2 v2)
     | Prod t1 t2 => exists v1 v2 : expr, v = Pair v1 v2 /\ V t1 v1 /\ V t2 v2
-    | Arrow t1 t2 => exists (e: {bind expr}), ((v = Abs e) /\ (forall (v': expr), V t1 v' -> E t2 (e .[v' .: ids])))
+    | Arrow t1 t2 => exists e: {bind expr}, v = Abs e /\ forall (v' : expr), V t1 v' -> E t2 (e .[v' .: ids])
     end.
 
   Definition E t e := exists v, (cbv_multi e v) /\ (V t v).
@@ -147,8 +183,10 @@ Module STLC.
   Proof.
     induction t; intros; inversion H.
     - apply value_null.
-    - destruct H0. subst v. apply value_abs.
-    - destruct H0 as [v2 [Eq [V1 V2]]]. subst v. apply value_pair; eauto.
+    - destruct H0. subst v. eauto.
+    - destruct H0 as [v2 [Eq [V1 V2]]]. subst v. eauto.
+    - destruct H0. destruct H0. apply IHt1 in H1. subst. eauto.
+    - destruct H0. destruct H0. apply IHt2 in H1. subst. eauto.
   Qed.
 
   (* Taken from line 239 of https://gist.github.com/tmoux/5027a9b9f6b5aee291d569e5f144b350#file-stlc-v-L8 *)
@@ -176,19 +214,19 @@ Module STLC.
   (** Fundamental theorem of logical relations *)
   Theorem fundamental_theorem : forall Γ e t, Γ ⊢ e ::: t -> Γ ⊨ e ::: t.
   Proof.
-    intros Γ e t H. induction H; unfold semant_typing; intros γ VS; unfold E; simpl.
+    intros Γ e t H. induction H; unfold semant_typing in *; intros γ VS; unfold E; simpl.
     (* pair *)
-    - unfold semant_typing in IHtyping1, IHtyping2. remember (IHtyping1 γ VS) as E1. remember (IHtyping2 γ VS) as E2. unfold E in E1, E2. destruct E1, E2. destruct a, a0. eexists (Pair x x0). split. apply pair_steps_steps_steps; auto. eauto.
+    - remember (IHtyping1 γ VS) as E1. remember (IHtyping2 γ VS) as E2. unfold E in E1, E2. destruct E1, E2. destruct a, a0. eexists (Pair x x0). split. apply pair_steps_steps_steps; auto. eauto.
     (* pi1 *)
-    - unfold semant_typing in IHtyping. remember (IHtyping γ VS) as E1. unfold E in E1. destruct E1. destruct a. inversion v. destruct H0 as [v2 [Eq [V1 V2]]]. exists x0. split; auto. eapply rtn1_trans. instantiate (1 := Pi1 (Pair x0 v2)). apply cbv_val_pi1. subst x. apply pi1_steps_steps. auto.
+    - remember (IHtyping γ VS) as E1. unfold E in E1. destruct E1. destruct a. inversion v. destruct H0 as [v2 [Eq [V1 V2]]]. exists x0. split; auto. eapply rtn1_trans. instantiate (1 := Pi1 (Pair x0 v2)). apply cbv_val_pi1. subst x. apply pi1_steps_steps. auto.
     (* pi2 *)
-    - unfold semant_typing in IHtyping. remember (IHtyping γ VS) as E1. unfold E in E1. destruct E1. destruct a. inversion v. destruct H0 as [v2 [Eq [V1 V2]]]. exists v2. split; auto. eapply rtn1_trans. instantiate (1 := Pi2 (Pair x0 v2)). apply cbv_val_pi2. subst x. apply pi2_steps_steps. auto.
+    - remember (IHtyping γ VS) as E1. unfold E in E1. destruct E1. destruct a. inversion v. destruct H0 as [v2 [Eq [V1 V2]]]. exists v2. split; auto. eapply rtn1_trans. instantiate (1 := Pi2 (Pair x0 v2)). apply cbv_val_pi2. subst x. apply pi2_steps_steps. auto.
     (* abs *)
-    - unfold semant_typing in IHtyping. exists (Abs e.[up γ]). split.
+    - exists (Abs e.[up γ]). split.
       + apply rtn1_refl.
-      + exists (e.[up γ]). split; auto. intros. Search "subst". specialize (IHtyping (v' .: γ)). assert (valid_subst (t1 :: Γ) (v' .: γ)) as lemma. { apply subst_cons; auto. } apply IHtyping in lemma. unfold E in lemma. autosubst.
+      + exists (e.[up γ]). split; auto. intros. specialize (IHtyping (v' .: γ)). assert (valid_subst (t1 :: Γ) (v' .: γ)) as lemma. { apply subst_cons; auto. } apply IHtyping in lemma. unfold E in lemma. autosubst.
     (* app *)
-    - unfold semant_typing in IHtyping1, IHtyping2. remember (IHtyping1 γ VS) as E1. remember (IHtyping2 γ VS) as E2. unfold E in E1, E2. destruct E1 as [v_fun [S1 V1]]. destruct E2 as [v_arg [S2 V2]]. inversion V1. destruct H1. subst v_fun. specialize (H2 v_arg). remember (H2 V2). destruct e as [v [Sv Vv]]. exists v. split.
+    - remember (IHtyping1 γ VS) as E1. remember (IHtyping2 γ VS) as E2. unfold E in E1, E2. destruct E1 as [v_fun [S1 V1]]. destruct E2 as [v_arg [S2 V2]]. inversion V1. destruct H1. subst v_fun. specialize (H2 v_arg). remember (H2 V2). destruct e as [v [Sv Vv]]. exists v. split.
       + apply cbv_multi_trans with (e' := App (Abs x) v_arg).
         * apply cbv_multi_trans with (e' := App (Abs x) (e2.[γ])).
           -- apply app_fun_steps_steps; auto.
@@ -197,6 +235,14 @@ Module STLC.
           -- apply Operators_Properties.clos_rtn1_step. apply cbv_sub. apply (V_implies_value t1). auto.
           -- auto.
       + auto.
+    (* inl *)
+    - remember (IHtyping γ VS). unfold E in e0. destruct e0 as [v [S V1]]. exists (Inl v). split; eauto using inl_steps_steps.
+    (* inr *)
+    - remember (IHtyping γ VS). unfold E in e0. destruct e0 as [v [S V2]]. exists (Inr v). split; eauto using inr_steps_steps.
+    (* case *)
+    - remember (IHtyping1 γ VS). unfold E in e0. destruct e0 as [v [S Vsum]]. inversion Vsum; destruct H2; destruct H2; subst.
+      + specialize (IHtyping2 (x .: γ)). apply subst_cons with (v := x) (t := t1) in VS as Hehe; try assumption. apply IHtyping2 in Hehe. unfold E in Hehe. destruct Hehe as [v [S' Vv]]. exists v. split; try assumption. apply cbv_multi_trans with (e' := Case (Inl x) e1.[up γ] e2.[up γ]). apply case_steps_steps. assumption. apply cbv_multi_trans with (e' := e1.[x .: γ]); auto. apply rtn1_trans with (y := Case (Inl x) e1.[up γ] e2.[up γ]); eauto. assert (e1.[up γ].[x/] = e1.[x .: γ]) as AS. { autosubst. } rewrite <- AS. eauto.
+      + specialize (IHtyping3 (x .: γ)). apply subst_cons with (v := x) (t := t2) in VS as Hehe; try assumption. apply IHtyping3 in Hehe. unfold E in Hehe. destruct Hehe as [v [S' Vv]]. exists v. split; try assumption. apply cbv_multi_trans with (e' := Case (Inr x) e1.[up γ] e2.[up γ]). apply case_steps_steps. assumption. apply cbv_multi_trans with (e' := e2.[x .: γ]); auto. apply rtn1_trans with (y := Case (Inr x) e1.[up γ] e2.[up γ]); eauto. assert (e2.[up γ].[x/] = e2.[x .: γ]) as AS. { autosubst. } rewrite <- AS. eauto.
     (* null *)
     - exists Null. split; auto. apply rtn1_refl.
     (* var *)
